src/Dflatmajor.v
@@ -11,6 +11,7 @@ Require Import compcert.common.Switch.
 (*Require Import compcert.common.Smallstep.*)
 Require Import TraceSemantics.
 Require Import HighValues.
+Require Import AllValues.
 
 Require Import List.
 Import ListNotations.
@@ -288,7 +289,8 @@ Inductive final_state (p : program) : state -> value -> Prop :=
 (** The corresponding small-step semantics. *)
 
 Definition semantics (p: program) :=
-  Semantics step (is_callstate p) (final_state p) (Genv.globalenv p).
+  Semantics (val_level := VlHigh)
+    step (is_callstate p) (final_state p) (Genv.globalenv p).
 
 (** This semantics is receptive to changes in events. *)
 
