src/Cmajortominor.v
@@ -506,27 +506,12 @@ Proof.
   intros.
   eapply TraceSemantics.forward_simulation_step with (match_states := match_states).
   instantiate (1 := eq).
-  intros. eapply is_callstate_match; eauto.
-  congruence.
-  intros. eapply match_final_state in H0; eauto.
-  eapply single_step_correct; eauto.
-Defined.
-
-Lemma match_val_eq :
-  TraceSemantics.fsim_match_val fsim = eq.
-Proof.
-  intros.
-  unfold fsim. simpl.
-  unfold TraceSemantics.fsim_match_val.
-  repeat break_match. repeat (break_match_hyp; try congruence).
-  
-  try unfold forward_simulation_step in *.
-  try unfold forward_simulation_plus in *.
-  try unfold forward_simulation_star in *.
-  try unfold forward_simulation_star_wf in *.
-  try inv Heqf. 
-  
-  reflexivity.
+  - intros. eapply is_callstate_match; eauto.
+    congruence.
+  - intros. eapply match_final_state in H0; eauto.
+  - simpl. auto.
+  - simpl. intros. tauto.
+  - eapply single_step_correct; eauto.
 Qed.
 
 
