src/OeufProof.v
@@ -1,5 +1,4 @@
 Require Import Oeuf.
-Require TopLevel.
 Require Import CompilationUnit.
 Require Import HList.
 Require Import StepLib.
